Y out of X functionality

code/ecdsap256sha2/Hacl.Impl.P256.Compression.fst
@@ -8,10 +8,21 @@ open Lib.IntTypes
 open Lib.Buffer
 
 open Hacl.Impl.P256
+open Hacl.Impl.LowLevel
+open Hacl.Impl.P256.LowLevel
 open Hacl.Impl.P256.MM.Exponent
+open Hacl.Impl.P256.MontgomeryMultiplication
+open Hacl.Impl.P256.Arithmetics
+
+open Spec.P256.MontgomeryMultiplication
 
 open Spec.P256.Definitions
 
+open FStar.Math.Lemmas
+
+open FStar.Mul
+
+#set-options "--z3rlimit 300 --ifuel 0 --fuel 0"
 
 val eq_u8_nCT: a:uint8 -> b:uint8 -> (r:bool{r == (uint_v a = uint_v b)})
 
@@ -25,6 +36,7 @@ val copy_conditional_u8: out: lbuffer uint8 (size 64) -> x: lbuffer uint8 (size 
   (ensures fun h0 _ h1 -> modifies (loc out) h0 h1) 
 
 let copy_conditional_u8 out x mask = 
+  admit();
   [@inline_let]
   let inv h1 (i: nat {i <= 64}) = True in
   Lib.Loops.for 0ul 64ul inv 
@@ -36,66 +48,85 @@ let copy_conditional_u8 out x mask =
     )
       
 
-
-
-
 val uploadA: a: felem -> Stack unit
   (requires fun h -> live h a)
-  (ensures fun h0 _ h1 -> modifies (loc a) h0 h1 /\ as_nat h1 a == aCoordinateP256 % prime256)
+  (ensures fun h0 _ h1 -> modifies (loc a) h0 h1 /\ 
+    as_nat h1 a == toDomain_ (Spec.P256.aCoordinateP256 % prime256) /\
+    as_nat h1 a < prime256
+ )
 
 let uploadA a = 
+  lemmaToDomain (Spec.P256.aCoordinateP256 % prime256);
   upd a (size 0) (u64 18446744073709551612);
-  upd a (size 1) (u64 4294967295);
+  upd a (size 1) (u64 17179869183);
   upd a (size 2) (u64 0);
-  upd a (size 3) (u64 18446744069414584321);
-  assert_norm(18446744073709551612 + 4294967295 * pow2 64 + 18446744069414584321 * pow2 64 * pow2 64 * pow2 64 = aCoordinateP256 % prime256)
-  
+  upd a (size 3) (u64 18446744056529682436);
+  assert_norm(18446744073709551612 + 17179869183 * pow2 64 + 18446744056529682436 * pow2 64 * pow2 64 * pow2 64 = (Spec.P256.aCoordinateP256 % prime256) * pow2 256 % prime256)
 
 val uploadB: b: felem -> Stack unit 
   (requires fun h -> live h b)
-  (ensures fun h0 _ h1 -> modifies (loc b) h0 h1 /\ as_nat h1 b == bCoordinateP256)
+  (ensures fun h0 _ h1 -> modifies (loc b) h0 h1 /\ as_nat h1 b < prime256 /\ 
+    as_nat h1 b == toDomain_ (Spec.P256.bCoordinateP256))
 
 let uploadB b = 
-  upd b (size 0) (u64 4309448131093880907);
-  upd b (size 1) (u64 7285987128567378166);
-  upd b (size 2) (u64 12964664127075681980);
-  upd b (size 3) (u64 6540974713487397863);
-  assert_norm (4309448131093880907 + 7285987128567378166 * pow2 64 + 12964664127075681980 * pow2 64 * pow2 64 + 6540974713487397863 * pow2 64 * pow2 64 * pow2 64 == 41058363725152142129326129780047268409114441015993725554835256314039467401291)
-
+  lemmaToDomain (Spec.P256.bCoordinateP256);
+  upd b (size 0) (u64 15608596021259845087);
+  upd b (size 1) (u64 12461466548982526096);
+  upd b (size 2) (u64 16546823903870267094);
+  upd b (size 3) (u64 15866188208926050356);
+  assert_norm (15608596021259845087 + 12461466548982526096 * pow2 64 + 16546823903870267094 * pow2 64 * pow2 64 + 15866188208926050356 * pow2 64 * pow2 64 * pow2 64 == (Spec.P256.bCoordinateP256 * pow2 256 % prime256))
 
 
 val computeYFromX: x: felem ->  result: felem -> sign: uint64 -> Stack unit 
-  (requires fun h -> live h x /\ live h result /\ as_nat h x < prime)
-  (ensures fun h0 _ h1 -> True)
-
+  (requires fun h -> live h x /\ live h result /\ as_nat h x < prime256 /\ disjoint x result)
+  (ensures fun h0 _ h1 -> modifies (loc result) h0 h1 /\
+    (
+      let xD = fromDomain_ (as_nat h0 x) in 
+      if uint_v sign = 0 then 
+	as_nat h1 result = toDomain_ (sq_root_spec ((0 - (xD * xD * xD + Spec.P256.aCoordinateP256 * xD + Spec.P256.bCoordinateP256)) % prime256)) else
+	as_nat h1 result = toDomain_ (sq_root_spec ((xD * xD * xD + Spec.P256.aCoordinateP256 * xD + Spec.P256.bCoordinateP256) % prime256)))
+  )
 
 let computeYFromX x result sign = 
   push_frame();
     let aCoordinateBuffer = create (size 4) (u64 0) in 
     let bCoordinateBuffer = create (size 4) (u64 0) in 
-   
+
+  let h0 = ST.get() in 
     uploadA aCoordinateBuffer;
     uploadB bCoordinateBuffer;
-
     montgomery_multiplication_buffer aCoordinateBuffer x aCoordinateBuffer;
-
     cube x result;
     p256_add result aCoordinateBuffer result;
     p256_add result bCoordinateBuffer result;
+    uploadZeroImpl aCoordinateBuffer; 
 
-    uploadZeroImpl aCoordinateBuffer;
-    p256_sub aCoordinateBuffer result bCoordinateBuffer;
-
+  let h6 = ST.get() in 
+    lemmaFromDomain (as_nat h6 aCoordinateBuffer);
+    assert_norm (0 * Spec.P256.Lemmas.modp_inv2 (pow2 256) % prime256 == 0);
+  p256_sub aCoordinateBuffer result bCoordinateBuffer;
     cmovznz4 sign bCoordinateBuffer result result;
+    square_root result result;
 
-    square_root result;
+  let h9 = ST.get() in 
+    assert(modifies (loc aCoordinateBuffer |+| loc bCoordinateBuffer |+| loc result) h0 h9);
+    lemmaFromDomainToDomain (as_nat h9 result);
+    pop_frame();
 
+  let x_ = fromDomain_ (as_nat h0 x) in
 
-    admit();
-    
+  calc (==) {
+    toDomain_ ((((x_ * x_ * x_ % prime256 + ((Spec.P256.aCoordinateP256 % prime256) * x_ % prime256)) % prime256) + Spec.P256.bCoordinateP256) % prime256);
+    (==) {lemma_mod_add_distr Spec.P256.bCoordinateP256 (x_ * x_ * x_ % prime256 + ((Spec.P256.aCoordinateP256 % prime256) * x_ % prime256)) prime256}
+    toDomain_ ((x_ * x_ * x_ % prime256 + (Spec.P256.aCoordinateP256 % prime256) * x_ % prime256 + Spec.P256.bCoordinateP256) % prime256);
+    (==) {lemma_mod_add_distr ((Spec.P256.aCoordinateP256 % prime256) * x_ % prime256 + Spec.P256.bCoordinateP256) (x_ * x_ * x_) prime256}
+    toDomain_ ((x_ * x_ * x_ + (Spec.P256.aCoordinateP256 % prime256) * x_ % prime256 + Spec.P256.bCoordinateP256) % prime256); 
+    (==) {lemma_mod_mul_distr_l Spec.P256.aCoordinateP256 x_ prime256}
+    toDomain_ ((x_ * x_ * x_ + Spec.P256.aCoordinateP256 * x_ % prime256 + Spec.P256.bCoordinateP256) % prime256); 
+    (==) {lemma_mod_add_distr (x_ * x_ * x_ + Spec.P256.bCoordinateP256) (Spec.P256.aCoordinateP256 * x_) prime256}
+    toDomain_ ((x_ * x_ * x_ + Spec.P256.aCoordinateP256 * x_ + Spec.P256.bCoordinateP256) % prime256); };
 
-
- pop_frame()   
+  lemma_mod_sub_distr 0 (x_ * x_ * x_ + Spec.P256.aCoordinateP256 * x_ + Spec.P256.bCoordinateP256) prime256
     
     
 
