code/ecdsap256sha2/Hacl.Impl.P256.DH.fst
@@ -13,6 +13,7 @@ open Spec.ECDSA
 open Spec.P256.Definitions
 open Spec.DH
 open Spec.ECDSAP256.Definition
+open Spec.P256.Lemmas
 
 open Hacl.Impl.LowLevel
 open Hacl.Impl.P256
