code/ecdsap256sha2/Hacl.Impl.P256.MM.Exponent.fsti
@@ -35,6 +35,7 @@ open Spec.P256.MontgomeryMultiplication
 val square_root: a: felem -> result: felem ->  Stack unit 
   (requires fun h -> live h a /\ live h result /\ as_nat h a < prime)
   (ensures fun h0 _ h1 -> modifies (loc a |+| loc result) h0 h1 /\
+    as_nat h1 result < prime /\
     fromDomain_ (as_nat h1 result) = sq_root_spec (fromDomain_ (as_nat h0 a)) /\
     fromDomain_ (as_nat h1 result) = pow (fromDomain_ (as_nat h0 a)) ((prime256 + 1) / 4) % prime256
   )
